src/Spec/Curve25519.v
@@ -69,54 +69,53 @@ Proof.
   native_cast_no_check (@eq_refl bool true).
 Time Qed. (* 1s *)
 
-Local Notation F := (F p).
 
 Require PrimeFieldTheorems.
 
-Lemma field : @Hierarchy.field F eq F.zero F.one F.opp F.add F.sub F.mul F.inv F.div.
-Proof. apply PrimeFieldTheorems.F.field_modulo, prime_p. Qed.
-Lemma char_ge_3 : @Ring.char_ge F eq F.zero F.one F.opp F.add F.sub F.mul 3.
-Proof. eapply Hierarchy.char_ge_weaken; try apply ModularArithmeticTheorems.F.char_gt; Decidable.vm_decide. Qed.
+Lemma field : @Hierarchy.field (Zmod p) eq Zmod.zero Zmod.one Zmod.opp Zmod.add Zmod.sub Zmod.mul Zmod.inv Zmod.mdiv.
+Proof. apply PrimeFieldTheorems.Zmod.field_modulo, prime_p. Qed.
+Lemma char_ge_3 : @Ring.char_ge (Zmod p) eq Zmod.zero Zmod.one Zmod.opp Zmod.add Zmod.sub Zmod.mul 3.
+Proof. eapply Hierarchy.char_ge_weaken; try apply ModularArithmeticTheorems.Zmod.char_gt; Decidable.vm_decide. Qed.
 
 Require Import Spec.CompleteEdwardsCurve.
 Module E.
-  Definition a : F := F.opp 1.
-  Definition d : F := F.div (F.opp (F.of_Z _ 121665)) (F.of_Z _ 121666).
+  Definition a : Zmod p := Zmod.opp 1.
+  Definition d : Zmod p := Zmod.mdiv (Zmod.opp (Zmod.of_Z _ 121665)) (Zmod.of_Z _ 121666).
 
-  Lemma nonzero_a : a <> F.zero. Proof. Decidable.vm_decide. Qed.
-  Lemma square_a : exists sqrt_a, F.mul sqrt_a sqrt_a = a.
-  Proof. epose (@PrimeFieldTheorems.F.Decidable_square p prime_p eq_refl); Decidable.vm_decide. Qed.
-  Lemma nonsquare_d : forall x, F.mul x x <> d.
-  Proof. epose (@PrimeFieldTheorems.F.Decidable_square p prime_p eq_refl); Decidable.vm_decide. Qed.
+  Lemma nonzero_a : a <> Zmod.zero. Proof. Decidable.vm_decide. Qed.
+  Lemma square_a : exists sqrt_a, Zmod.mul sqrt_a sqrt_a = a.
+  Proof. epose (@PrimeFieldTheorems.Zmod.Decidable_square p prime_p eq_refl); Decidable.vm_decide. Qed.
+  Lemma nonsquare_d : forall x, Zmod.mul x x <> d.
+  Proof. epose (@PrimeFieldTheorems.Zmod.Decidable_square p prime_p eq_refl); Decidable.vm_decide. Qed.
 
-  Definition point := @E.point F eq F.one F.add F.mul a d.
+  Definition point := @E.point (Zmod p) eq Zmod.one Zmod.add Zmod.mul a d.
   Definition add := E.add(field:=field)(char_ge_3:=char_ge_3)(a:=a)(d:=d)
     (nonzero_a:=nonzero_a)(square_a:=square_a)(nonsquare_d:=nonsquare_d).
   Definition zero := E.zero(field:=field)(a:=a)(d:=d)(nonzero_a:=nonzero_a).
   Definition B : E.point.
     refine (
-    exist _ (F.of_Z _ 15112221349535400772501151409588531511454012693041857206046113283949847762202, F.div (F.of_Z _ 4) (F.of_Z _ 5)) _).
+    exist _ (Zmod.of_Z _ 15112221349535400772501151409588531511454012693041857206046113283949847762202, Zmod.mdiv (Zmod.of_Z _ 4) (Zmod.of_Z _ 5)) _).
     Decidable.vm_decide.
   Defined.
 End E.
 
 Require Import Spec.MontgomeryCurve.
 Module M.
-  Definition a : F := F.of_Z _ 486662.
-  Definition b : F := F.one.
-  Definition a24 : F := ((a - F.of_Z _ 2) / F.of_Z _ 4)%F.
-  Definition point := @M.point F eq F.add F.mul a b.
+  Definition a : Zmod p := Zmod.of_Z _ 486662.
+  Definition b : Zmod p := Zmod.one.
+  Definition a24 : Zmod p := ((a - Zmod.of_Z _ 2) / Zmod.of_Z _ 4)%Zmod.
+  Definition point := @M.point (Zmod p) eq Zmod.add Zmod.mul a b.
   Definition B : point :=
-    exist _ (inl (F.of_Z _ 9, F.of_Z _ 14781619447589544791020593568409986887264606134616475288964881837755586237401)) eq_refl.
+    exist _ (inl (Zmod.of_Z _ 9, Zmod.of_Z _ 14781619447589544791020593568409986887264606134616475288964881837755586237401)) eq_refl.
 
-  Lemma a2m4_nonzero : F.sub (F.mul a a) (F.of_Z _ 4) <> F.zero. Decidable.vm_decide. Qed.
-  Lemma a2m4_nonsq : ~(exists r, F.mul r r = F.sub (F.mul a a) (F.of_Z _ 4)).
-  Proof. epose (@PrimeFieldTheorems.F.Decidable_square p prime_p eq_refl); Decidable.vm_decide. Qed.
-  Lemma b_nonzero : b <> F.zero. Decidable.vm_decide. Qed.
+  Lemma a2m4_nonzero : Zmod.sub (Zmod.mul a a) (Zmod.of_Z _ 4) <> Zmod.zero. Decidable.vm_decide. Qed.
+  Lemma a2m4_nonsq : ~(exists r, Zmod.mul r r = Zmod.sub (Zmod.mul a a) (Zmod.of_Z _ 4)).
+  Proof. epose (@PrimeFieldTheorems.Zmod.Decidable_square p prime_p eq_refl); Decidable.vm_decide. Qed.
+  Lemma b_nonzero : b <> Zmod.zero. Decidable.vm_decide. Qed.
 
   Definition add := (M.add(field:=field)(char_ge_3:=char_ge_3)(a:=a)(b_nonzero:=b_nonzero)).
   Definition opp := (M.opp(field:=field)(a:=a)(b_nonzero:=b_nonzero)).
-  Definition X0 := (M.X0(Feq:=eq)(Fzero:=F.zero)(Fadd:=F.add)(Fmul:=F.mul)(a:=a)(b:=b)).
+  Definition X0 := (M.X0(Feq:=eq)(Fzero:=Zmod.zero)(Fadd:=Zmod.add)(Fmul:=Zmod.mul)(a:=a)(b:=b)).
   Definition scalarmult := (@ScalarMult.scalarmult_ref _ add M.zero opp).
 End M.
 
