src/Spec/Test/X25519.v
@@ -4,34 +4,34 @@
 From Coq Require Import ZArith.
 Require Import Spec.ModularArithmetic Spec.Curve25519 Spec.MxDH Crypto.Util.Decidable.
 Definition cswap {T} (swap:bool) (a b:T) := if swap then (b, a) else (a, b).
-Definition monty s : F p -> F p := @MxDH.montladder _ F.zero F.one F.add F.sub F.mul F.inv M.a24 cswap 255 (fun i => Z.testbit s (Z.of_nat i)).
+Definition monty s : Zmod p -> Zmod p := @MxDH.montladder _ Zmod.zero Zmod.one Zmod.add Zmod.sub Zmod.mul Zmod.inv M.a24 cswap 255 (fun i => Z.testbit s (Z.of_nat i)).
 
-Example one_basepoint : F.to_Z (monty 1 (F.of_Z _ 9)) = 9%Z.
+Example one_basepoint : Zmod.unsigned (monty 1 (Zmod.of_Z _ 9)) = 9%Z.
 Proof. vm_decide_no_check. Qed.
 
-Example testvector_one : F.to_Z (monty
+Example testvector_one : Zmod.unsigned (monty
    31029842492115040904895560451863089656472772604678260265531221036453811406496%Z
-   (F.of_Z _ 34426434033919594451155107781188821651316167215306631574996226621102155684838%Z)) = 37325765543539916631701301279660700968428932651319597985674090122993663859395%Z.
+   (Zmod.of_Z _ 34426434033919594451155107781188821651316167215306631574996226621102155684838%Z)) = 37325765543539916631701301279660700968428932651319597985674090122993663859395%Z.
 Proof. vm_decide_no_check. Qed.
 
-Example testvector_two : F.to_Z (monty
+Example testvector_two : Zmod.unsigned (monty
    35156891815674817266734212754503633747128614016119564763269015315466259359304%Z
-   (F.of_Z _ 8883857351183929894090759386610649319417338800022198945255395922347792736741%Z)) = 39566196721700740701373067725336211924689549479508623342842086701180565506965%Z.
+   (Zmod.of_Z _ 8883857351183929894090759386610649319417338800022198945255395922347792736741%Z)) = 39566196721700740701373067725336211924689549479508623342842086701180565506965%Z.
 Proof. vm_decide_no_check. Qed.
 
-Example order_basepoint : F.to_Z (monty l (F.of_Z _ 9)) = 0%Z.
+Example order_basepoint : Zmod.unsigned (monty l (Zmod.of_Z _ 9)) = 0%Z.
 Proof. vm_decide_no_check. Qed. (* note: ideally we'd check that z=0 *)
 
 Definition double x := (* takes as input affine x, returns projective x/z *)
-  fst (@MxDH.ladderstep _ F.add F.sub F.mul M.a24 (F.of_Z _ 0) (x, F.of_Z _ 1) (x, F.of_Z _ 1)).
+  fst (@MxDH.ladderstep _ Zmod.add Zmod.sub Zmod.mul M.a24 (Zmod.of_Z _ 0) (x, Zmod.of_Z _ 1) (x, Zmod.of_Z _ 1)).
 (* EllipticCurve(GF(2^255 - 19), [0,486662,0,1,0]).torsion_polynomial(8).roots(multiplicities=False) *)
 (* Point of order 2: *)
-Lemma double_zero : snd (double (F.of_Z _ 0)) = F.of_Z _ 0. vm_decide_no_check. Qed.
+Lemma double_zero : snd (double (Zmod.of_Z _ 0)) = Zmod.of_Z _ 0. vm_decide_no_check. Qed.
 (* Points of order 4: *)
-Lemma double_one  : fst (double (F.of_Z _ 1)) = F.of_Z _ 0. vm_decide_no_check. Qed.
-Lemma double_minusone:fst(double(F.of_Z _(-1)))=F.of_Z _ 0. vm_decide_no_check. Qed.
+Lemma double_one  : fst (double (Zmod.of_Z _ 1)) = Zmod.of_Z _ 0. vm_decide_no_check. Qed.
+Lemma double_minusone:fst(double(Zmod.of_Z _(-1)))=Zmod.of_Z _ 0. vm_decide_no_check. Qed.
 (* Points of order 8: *)
-Definition order8_x1 := F.of_Z p 39382357235489614581723060781553021112529911719440698176882885853963445705823.
-Definition order8_x2 := F.of_Z p 325606250916557431795983626356110631294008115727848805560023387167927233504.
+Definition order8_x1 := Zmod.of_Z p 39382357235489614581723060781553021112529911719440698176882885853963445705823.
+Definition order8_x2 := Zmod.of_Z p 325606250916557431795983626356110631294008115727848805560023387167927233504.
 Lemma double_order8_x1 : fst (double order8_x1) = snd (double order8_x1). vm_decide_no_check. Qed.
 Lemma double_order8_x2 : fst (double order8_x2) = snd (double order8_x2). vm_decide_no_check. Qed.
