src/Spec/ModularArithmetic.v
@@ -1,45 +1,19 @@
 From Coq Require Import BinIntDef.
 From Coq Require Import BinNatDef.
 From Coq Require Import BinPosDef.
-From Coq Require Import Zmod.
+From Coq Require Export Zmod.
 
 Global Coercion BinInt.Z.pos : BinPos.positive >-> BinInt.Z.
 Global Coercion BinInt.Z.of_N : BinNums.N >-> BinInt.Z.
 Global Coercion Zmod.unsigned : Zmod.Zmod >-> BinInt.Z.
 Global Set Printing Coercions.
 
-Notation F := Zmod.Zmod (only parsing).
-Module F.
-  Notation of_Z := Zmod.of_Z (only parsing).
-  Notation to_Z := Zmod.unsigned (only parsing).
-  Notation zero := Zmod.zero (only parsing).
-  Notation one := Zmod.one (only parsing).
-  Notation add := Zmod.add (only parsing).
-  Notation sub := Zmod.sub (only parsing).
-  Notation mul := Zmod.mul (only parsing).
-  Notation opp := Zmod.opp (only parsing).
-  Notation inv := Zmod.inv (only parsing).
-  Notation div := Zmod.mdiv (only parsing).
-  Notation pow := Zmod.pow (only parsing).
+Infix "/" := Zmod.mdiv : Zmod_scope.
 
-  Definition of_nat m (n:nat) := F.of_Z m (BinInt.Z.of_nat n).
-  Definition to_nat {m} (x:F m) := BinInt.Z.to_nat (F.to_Z x).
-  Notation nat_mod := of_nat (only parsing).
+Module Zmod.
+  Definition of_nat m (n:nat) := Zmod.of_Z m (BinInt.Z.of_nat n).
+  Definition to_nat {m} (x:Zmod m) := BinInt.Z.to_nat (Zmod.unsigned x).
 
-  Definition of_N m n := F.of_Z m (BinInt.Z.of_N n).
-  Definition to_N {m} (x:F m) := BinInt.Z.to_N (F.to_Z x).
-  Notation N_mod := of_N (only parsing).
-
-  Notation Z_mod := of_Z (only parsing).
-End F.
-
-Declare Scope F_scope.
-Delimit Scope F_scope with F.
-Bind Scope F_scope with Zmod.Zmod.
-Infix "+" := F.add : F_scope.
-Infix "*" := F.mul : F_scope.
-Infix "-" := F.sub : F_scope.
-Infix "/" := F.div : F_scope.
-Infix "^" := F.pow : F_scope.
-Notation "0" := F.zero : F_scope.
-Notation "1" := F.one : F_scope.
+  Definition of_N m n := Zmod.of_Z m (BinInt.Z.of_N n).
+  Definition to_N {m} (x:Zmod m) := BinInt.Z.to_N (Zmod.unsigned x).
+End Zmod.
